WIP addMemoryBlock: add chained free slots list and nodup consistency properties + propagate pdentry in modified state

proof/StateLib.v
@@ -488,6 +488,48 @@ Definition getChildren (partition : paddr) s :=
 	|_ => []
 end.
 
+(** The [geTrdShadows] returns physical pages used to keep informations about
+    configuration pages
+*)
+Definition getFreeSlotsListAux bound FuncAux (blockentryaddr : paddr) s  : list optionPaddr:=
+match bound with
+|0 => [NonePaddr]
+|S bound1 => match lookup blockentryaddr s.(memory) beqAddr with
+						| Some (BE entry) => if entry.(blockrange).(endAddr) =? nullAddr then [SomePaddr blockentryaddr] else SomePaddr blockentryaddr :: FuncAux bound1 entry.(blockrange).(endAddr) s
+            |_ => [NonePaddr]
+           end
+end.
+
+Fixpoint getFreeSlotsListRec (bound : nat) (blockentryaddr : paddr) s {struct bound} := getFreeSlotsListAux bound getFreeSlotsListRec blockentryaddr s.
+
+(*Fixpoint getFreeSlotsListAux (blockentryaddr : paddr) s bound :=
+match bound with
+|0 => []
+|S bound1 => match lookup blockentryaddr s.(memory) beqAddr with
+						| Some (BE entry) => if entry.(blockrange).(endAddr) =? nullAddr then [blockentryaddr] else blockentryaddr :: getFreeSlotsListAux entry.(blockrange).(endAddr) s bound1
+            |_ => []
+           end
+end.*)
+
+Definition getFreeSlotsList (partition : paddr) s :=
+  match lookup partition s.(memory) beqAddr with
+  | Some (PDT pdentry) => getFreeSlotsListRec N pdentry.(firstfreeslot) s
+	|_ => []
+end.
+
+Fixpoint wellFormedFreeSlotsList (l : list optionPaddr) (s : state) :=
+match l with
+| [] => True
+| SomePaddr entryaddr :: l1 => wellFormedFreeSlotsList l1 s
+| _ => (* undef because of recursion *) False
+end.
+
+Lemma FreeSlotsListRec_unroll :
+forall blockentryaddr s bound, getFreeSlotsListRec bound blockentryaddr s = getFreeSlotsListAux bound getFreeSlotsListRec blockentryaddr s.
+destruct bound; simpl;reflexivity.
+Qed.
+
+
 (*
 (** The [getPartitionsAux] function returns all pages marked as descriptor partition *)
 Fixpoint getPartitionAux (partitionRoot : page) (s : state) bound {struct bound} : list page :=
@@ -575,14 +617,13 @@ end.
 (*DUP*)
 (** The [isSHE] proposition reutrns True if the entry at position [idx]
     into the given page [table] is type of [PE] *)
-(*Definition isFreeSlot paddr s: Prop := 
+Definition isFreeSlot paddr s: Prop :=
 match lookup paddr s.(memory) beqAddr with 
 |Some (BE entry) => match lookup (CPaddr (paddr + sh1offset)) s.(memory) beqAddr with
 									 	|Some (SHE sh1entry) =>
 												match lookup (CPaddr (paddr + scoffset)) s.(memory) beqAddr with 
 												|Some (SCE scentry) => entry.(blockrange).(startAddr) = nullAddr /\
-																							(* no cycles for same slot -> replace by general property on chained free slots if necessary*)
-																							(entry.(blockrange).(endAddr) <> nullAddr -> entry.(blockrange).(endAddr) <> paddr /\ isBE entry.(blockrange).(endAddr) s)  /\
+																							(* no cycles for same slot by general consistency property on chained free slots*)
 																							sh1entry.(PDchild) = nullAddr /\ sh1entry.(PDflag) = false /\ sh1entry.(inChildLocation) = nullAddr /\
 																							scentry.(origin) = nullAddr /\ scentry.(next) = nullAddr
 									 			|_ => False
@@ -590,38 +631,7 @@ match lookup paddr s.(memory) beqAddr with
 										|_ => False
 										end
 |_ => False
-end.*)
-
-Definition isFreeSlotChain (count : nat) f paddr (s : state) : Prop := 
-match count with
-| O => True
-| S n => match lookup paddr s.(memory) beqAddr with 
-				|Some (BE entry) => match lookup (CPaddr (paddr + sh1offset)) s.(memory) beqAddr with
-													 	|Some (SHE sh1entry) =>
-																match lookup (CPaddr (paddr + scoffset)) s.(memory) beqAddr with 
-																|Some (SCE scentry) => entry.(blockrange).(startAddr) = nullAddr /\
-																											(* no cycles for same slot -> replace by general property on chained free slots if necessary*)
-																											(entry.(blockrange).(endAddr) <> nullAddr -> entry.(blockrange).(endAddr) <> paddr /\ f n entry.(blockrange).(endAddr) s)  /\
-																											sh1entry.(PDchild) = nullAddr /\ sh1entry.(PDflag) = false /\ sh1entry.(inChildLocation) = nullAddr /\
-																											scentry.(origin) = nullAddr /\ scentry.(next) = nullAddr
-													 			|_ => False
-																end
-														|_ => False
-													end
-			|_ => False
-			end
 end.
-
-Fixpoint isFreeSlotAux (count : nat) paddr s: Prop := 
-isFreeSlotChain count isFreeSlotAux paddr s.
-
-Lemma funroll  :forall x paddr s, isFreeSlotAux x paddr s = isFreeSlotChain x isFreeSlotAux paddr s.
-destruct x ; simpl ; reflexivity.
-Qed.
-
-Definition isFreeSlot paddr (s : state) : Prop := 
-isFreeSlotAux N paddr s.
-
 
 (** The [entryUserFlag] proposition reutrns True if the entry at position [idx]
     into the given physical page [table] is type of [VE] and the user flag stored into 
