proof/InternalLemmas.v
@@ -35,8 +35,8 @@
     This file contains several internal lemmas to help prove invariants *)
 Require Import Model.ADT Model.Monad Model.MAL Model.Lib Core.Internal.
 
-(*Require Import Proof.Isolation Proof.Consistency Proof.WeakestPreconditions Proof.StateLib.
-Require Import Proof.DependentTypeLemmas Proof.Lib.
+(*Require Import Proof.Isolation Proof.Consistency Proof.WeakestPreconditions Proof.StateLib.*)
+Require Import DependentTypeLemmas. (*Proof.Lib.
 Require Import PropagatedProperties Invariants.*)
 
 Require Import List Coq.Logic.ProofIrrelevance Lia Classical_Prop Compare_dec EqNat Lt Minus.
@@ -8145,6 +8145,82 @@ Proof.
 unfold beqAddr. rewrite PeanoNat.Nat.eqb_refl. trivial.
 Qed.
 
+(*Lemma CPaddrInjection addr1 addr2 :
+addr1 <= maxAddr -> addr2 <= maxAddr
+-> CPaddr addr1 = CPaddr addr2 -> addr1 = addr2.
+Proof.
+intros. unfold CPaddr in *.
+destruct (le_dec addr1 maxAddr) eqn: Hj ; try congruence.
+destruct (le_dec addr2 maxAddr) eqn: Hk ; try congruence.
+Qed.*)
+
+Lemma CPaddrInjection3 addr1 :
+forall value1 s,
+lookup addr1 (memory s) beqAddr = value1 ->
+addr1 <= maxAddr.
+Proof.
+intros.
+destruct addr1. simpl in *. intuition.
+Qed.
+
+
+Lemma CPaddrInjection (addr1 addr2 : paddr):
+(*forall value1 value2 s,
+lookup addr1 (memory s) beqAddr = value1 ->
+lookup addr2 (memory s) beqAddr = value2 ->*)
+CPaddr addr1 = CPaddr addr2 -> addr1 = addr2.
+Proof.
+intros. (*
+apply CPaddrInjection3 in H.
+apply CPaddrInjection3 in H0.*)
+rewrite paddrEqId in H. rewrite paddrEqId in H. intuition.
+Qed.
+
+Lemma CPaddrInjectionNat (addr1nat addr2nat : nat) :
+addr1nat = addr2nat ->
+CPaddr addr1nat = CPaddr addr2nat.
+Proof.
+intros. rewrite H in *. reflexivity.
+Qed.
+
+
+Lemma CPaddrInjectionNat2 (addr1nat addr2nat : nat) :
+CPaddr addr1nat <> paddr_d -> CPaddr addr2nat <> paddr_d ->
+CPaddr addr1nat = CPaddr addr2nat ->
+addr1nat = addr2nat.
+Proof.
+intros.
+unfold CPaddr in * |-.
+destruct(le_dec addr1nat maxAddr) eqn:Hj.
+* destruct (le_dec addr2nat maxAddr) eqn:Hk.
+	** injection H1. intuition.
+	** congruence.
+* congruence.
+Qed.
+
+Lemma CPaddrInjection4 (addr1 : paddr):
+forall value1 s,
+lookup addr1 (memory s) beqAddr = value1 ->
+exists x, x = CPaddr addr1.
+Proof.
+intros.
+eexists. intuition.
+Qed.
+
+Lemma CPaddrInjection7 (addr1 addr2: paddr) :
+CPaddr addr1 <> CPaddr addr2 ->
+(p addr1) <> (p addr2).
+Proof.
+intros. intuition.
+Qed.
+
+Lemma CPaddrInjection6 (addr1 addr2: paddr) :
+CPaddr addr1 = CPaddr addr2 ->
+addr1 = addr2.
+Proof.
+intuition.
+apply CPaddrInjection. intuition.
+Qed.
 
 (*
 Lemma eqListTrueEq  :
